Risc0/Gadgets/IsZero/Witness/Code.lean
@@ -6,50 +6,80 @@ namespace Risc0.IsZero.Witness.Code
 open MLIRNotation
 
 def full : MLIRProgram :=
-  "1"         ←ₐ .Const 1;
-  "x"         ←ₐ Op.Get ⟨"input"⟩ 0 0;
+  let one := 0
+  let x := 1
+  let isZeroBit := 2
+  let invVal := 3
+  let arg10 := 4
+  let oneMinusArg10 := 5
+  let arg11 := 6
+  let xTimesArg11 := 7
+  let xTimesArg11Minus1 := 8
+  one         ←ₐ .Const 1;
+  x         ←ₐ Op.Get ⟨Input⟩ 0 0;
   nondet (
-    "isZeroBit" ←ₐ ??₀⟨"x"⟩;
-    ⟨"output"⟩[0]   ←ᵢ ⟨"isZeroBit"⟩;
-    "invVal"    ←ₐ Inv ⟨"x"⟩;
-    ⟨"output"⟩[1]   ←ᵢ ⟨"invVal"⟩  
+    isZeroBit ←ₐ ??₀⟨x⟩;
+    ⟨Output⟩[0]   ←ᵢ ⟨isZeroBit⟩;
+    invVal    ←ₐ Inv ⟨x⟩;
+    ⟨Output⟩[1]   ←ᵢ ⟨invVal⟩  
   );
-  "arg1[0]"   ←ₐ .Get ⟨"output"⟩ 0 0;
-  guard ⟨"arg1[0]"⟩ then
-    ?₀ ⟨"x"⟩;
-  "1 - arg1[0]" ←ₐ .Sub ⟨"1"⟩ ⟨"arg1[0]"⟩;
-  guard ⟨"1 - arg1[0]"⟩ then
-    "arg1[1]"        ←ₐ .Get ⟨"output"⟩ 0 1;
-    "x * arg1[1]"     ←ₐ .Mul ⟨"x"⟩ ⟨"arg1[1]"⟩;
-    "x * arg1[1] - 1" ←ₐ .Sub ⟨"x * arg1[1]"⟩ ⟨"1"⟩;
-    ?₀ ⟨"x * arg1[1] - 1"⟩
+  arg10   ←ₐ .Get ⟨Output⟩ 0 0;
+  guard ⟨arg10⟩ then
+    ?₀ ⟨x⟩;
+  oneMinusArg10 ←ₐ .Sub ⟨one⟩ ⟨arg10⟩;
+  guard ⟨oneMinusArg10⟩ then
+    arg11        ←ₐ .Get ⟨Output⟩ 0 1;
+    xTimesArg11     ←ₐ .Mul ⟨x⟩ ⟨arg11⟩;
+    xTimesArg11Minus1 ←ₐ .Sub ⟨xTimesArg11⟩ ⟨one⟩;
+    ?₀ ⟨xTimesArg11Minus1⟩
 
 def run (st: State) : BufferAtTime :=
   full.runProgram st |>.lastOutput
 
 def part₀ : MLIRProgram :=
-  "1" ←ₐ .Const 1;
-  "x" ←ₐ Op.Get ⟨"input"⟩ 0 0
+  let one := 0
+  let x := 1
+  one         ←ₐ .Const 1;
+  x         ←ₐ Op.Get ⟨Input⟩ 0 0
 
-def part₁ : MLIRProgram := nondet (
-    "isZeroBit" ←ₐ ??₀⟨"x"⟩;
-    ⟨"output"⟩[0]   ←ᵢ ⟨"isZeroBit"⟩;
-    "invVal"    ←ₐ Inv ⟨"x"⟩;
-    ⟨"output"⟩[1]   ←ᵢ ⟨"invVal"⟩  
+def part₁ : MLIRProgram := 
+  let x := 1
+  let isZeroBit := 2
+  let invVal := 3
+  nondet (
+    isZeroBit ←ₐ ??₀⟨x⟩;
+    ⟨Output⟩[0]   ←ᵢ ⟨isZeroBit⟩;
+    invVal    ←ₐ Inv ⟨x⟩;
+    ⟨Output⟩[1]   ←ᵢ ⟨invVal⟩  
   )
 
-def part₂ : MLIRProgram := "arg1[0]" ←ₐ .Get ⟨"output"⟩ 0 0
+def part₂ : MLIRProgram := 
+  let arg10 := 4
+  arg10   ←ₐ .Get ⟨Output⟩ 0 0
 
-def part₃ : MLIRProgram := guard ⟨"arg1[0]"⟩ then ?₀ ⟨"x"⟩
+def part₃ : MLIRProgram := 
+  let x := 1
+  let arg10 := 4
+  guard ⟨arg10⟩ then ?₀ ⟨x⟩
 
-def part₄ : MLIRProgram := "1 - arg1[0]" ←ₐ .Sub ⟨"1"⟩ ⟨"arg1[0]"⟩
+def part₄ : MLIRProgram := 
+  let one := 0
+  let arg10 := 4
+  let oneMinusArg10 := 5
+  oneMinusArg10 ←ₐ .Sub ⟨one⟩ ⟨arg10⟩
 
 def part₅ : MLIRProgram :=
-  guard ⟨"1 - arg1[0]"⟩ then
-    "arg1[1]"        ←ₐ .Get ⟨"output"⟩ 0 1;
-    "x * arg1[1]"     ←ₐ .Mul ⟨"x"⟩ ⟨"arg1[1]"⟩;
-    "x * arg1[1] - 1" ←ₐ .Sub ⟨"x * arg1[1]"⟩ ⟨"1"⟩;
-    ?₀ ⟨"x * arg1[1] - 1"⟩
+  let one := 0
+  let x := 1
+  let oneMinusArg10 := 5
+  let arg11 := 6
+  let xTimesArg11 := 7
+  let xTimesArg11Minus1 := 8
+  guard ⟨oneMinusArg10⟩ then
+    arg11        ←ₐ .Get ⟨Output⟩ 0 1;
+    xTimesArg11     ←ₐ .Mul ⟨x⟩ ⟨arg11⟩;
+    xTimesArg11Minus1 ←ₐ .Sub ⟨xTimesArg11⟩ ⟨one⟩;
+    ?₀ ⟨xTimesArg11Minus1⟩
 
 abbrev parts_combined : MLIRProgram :=
   part₀; part₁; part₂; part₃; part₄; part₅
